src/example/TreiberClient01.v
@@ -1,0 +1,123 @@
+From sflib Require Import sflib.
+From Paco Require Import paco.
+Require Import Coq.Classes.RelationClasses Lia Program.
+From Fairness Require Import pind Axioms ITreeLib Red TRed IRed2 WFLibLarge.
+From Fairness Require Import FairBeh Mod Concurrency Linking.
+From Fairness Require Import PCM IProp IPM IPropAux.
+From Fairness Require Import IndexedInvariants OpticsInterp SimWeakest.
+From Fairness Require Import TemporalLogic SCMemSpec TreiberStack AuthExclAnysRA.
+
+Module TreiberClient1.
+
+  Definition gvs : list nat := [1].
+  Definition s : SCMem.val := SCMem.val_ptr (0, 0).
+
+  Section CODE.
+
+    Definition state := unit.
+    Definition ident := void.
+
+    Definition push_two :
+      ktree (threadE ident state) unit unit
+      :=
+      fun _ =>
+        _ <- (trigger Yield;;; TreiberStack.push (s,(SCMem.val_nat 0)));;
+        _ <- (trigger Yield;;; TreiberStack.push (s,(SCMem.val_nat 1)));;
+        _ <- trigger Yield;;
+      Ret tt.
+
+    Definition omod : Mod.t :=
+      Mod.mk
+        tt
+        (Mod.get_funs [("push_two", Mod.wrap_fun push_two)])
+    .
+
+    Definition module : Mod.t :=
+      OMod.close
+        (omod)
+        (SCMem.mod gvs)
+    .
+
+  End CODE.
+
+End TreiberClient1.
+
+Section SPEC.
+
+  Context {src_state : Type}.
+  Context {src_ident : Type}.
+  Notation tgt_state := (Mod.state TreiberClient1.module).
+  Notation tgt_ident := (Mod.ident TreiberClient1.module).
+
+  Local Instance STT : StateTypes := Build_StateTypes src_state tgt_state src_ident tgt_ident.
+  Context `{sub : @SRA.subG Γ Σ}.
+  Context {TLRASs : TLRAs_small STT Γ}.
+  Context {TLRAS : TLRAs STT Γ Σ}.
+
+  Context {HasMemRA: @GRA.inG memRA Γ}.
+  Context {HasAuthExclAnysRA : @GRA.inG AuthExclAnysRA Γ}.
+
+  Ltac red_tl_all := red_tl; red_tl_memra; red_tl_auexa.
+
+  Import TreiberClient1.
+
+  Lemma push_two_spec
+        tid n
+        (* (TOP : OwnEs_top E) *)
+    :
+    ⊢ ∀ γs L (ds : list (nat * nat * sProp n)),
+    [@ tid, n, ⊤ @]
+      ⧼⟦(
+        (syn_tgt_interp_as n sndl (fun m => s_memory_black m)) ∗
+        (⤉ IsTreiber n s γs) ∗
+        (⤉ ○ γs ([] : list SCMem.val)) ∗
+        (⤉ Duty(tid) ds) ∗
+        ◇{List.map fst ds}(2 + L, 3)
+        )%S, 1+n⟧⧽
+        (OMod.close_itree omod (SCMem.mod gvs) (TreiberClient1.push_two tt))
+        ⧼_, ⟦(
+          (⤉ Duty(tid) ds) ∗
+          (⤉ ○ γs [SCMem.val_nat 1;SCMem.val_nat 0])
+        )%S, 1+n⟧⧽
+  .
+  Proof.
+    iIntros. iStartTriple.
+    red_tl_all. rewrite red_syn_tgt_interp_as; simpl.
+    iIntros "(#Mem & #IsTStack & TStack & Duty &Pcs)".
+    iMod (pcs_decr _ _ 2 1 with "Pcs") as "[Pcs PcsPush]"; [lia|].
+    iMod (pcs_decr _ _ 1 1 with "Pcs") as "[Pcs PcsPush']"; [lia|].
+    iMod (pcs_drop _ _ _ _ 1 100 with "Pcs") as "Pcs"; [lia|]. Unshelve. 2:lia.
+    iIntros "Post".
+    unfold push_two. rred.
+    iApply (wpsim_yieldR2 with "[$Duty $Pcs]"); [lia..|].
+    iIntros "Duty _ Pcs". rred2r. iApply wpsim_tauR. rred2r.
+    iApply (Treiber_push_spec _ (λ v, (○ γs [SCMem.val_nat 0]))%S with "[Duty PcsPush TStack] [-]"); [ss..| |].
+    { red_tl_all. rewrite red_syn_tgt_interp_as. iSplit; [eauto|]. iSplitR; [iFrame "#"|].
+      iFrame. iIntros (s_st). red_tl_all. iIntros "[TStackInv _]". simpl.
+      iDestruct (auexa_b_w_eq with "TStackInv TStack") as "%EQ".
+      subst s_st.
+      iMod (auexa_b_w_update with "TStackInv TStack") as "[TStackInv TStack]".
+      iModIntro. iFrame.
+    }
+    iEval (red_tl_all;simpl). iIntros (_) "[TStack Duty]".
+    rred2r.
+    iApply (wpsim_yieldR2 with "[$Duty $Pcs]"); [lia..|].
+    iIntros "Duty _ Pcs". rred2r.
+    iApply wpsim_tauR. rred2r.
+    iApply (Treiber_push_spec _ (λ v, ○ γs [SCMem.val_nat 1; SCMem.val_nat 0])%S with "[Duty PcsPush' TStack] [-]"); [ss..| |].
+    { red_tl_all. rewrite red_syn_tgt_interp_as. iSplit; [eauto|]. iSplitR; [iFrame "#"|].
+      iFrame. iIntros (s_st). red_tl_all. iIntros "[TStackInv _]". simpl.
+      iDestruct (auexa_b_w_eq with "TStackInv TStack") as "%EQ".
+      subst s_st.
+      iMod (auexa_b_w_update with "TStackInv TStack") as "[TStackInv TStack]".
+      iModIntro. iFrame.
+    }
+    iEval (red_tl_all;simpl). iIntros (_) "[TStack Duty]".
+    rred2r.
+    iApply (wpsim_yieldR2 with "[$Duty $Pcs]"); [lia..|].
+    iIntros "Duty _ Pcs". rred2r.
+    iApply wpsim_tauR. rred2r.
+    iApply "Post". iFrame.
+  Qed.
+
+End SPEC.
